WellFormed2.v
@@ -17,11 +17,131 @@ Require Import WellFormed.
 Module NatMapFacts := NatMapProperties.F.
 Module CacheletMapFacts := CacheletMapProperties.F.
 
+(* Disjoint VPT (used in wf3) *)
 Definition disjoint_VPT (V: VPT): Prop :=
   forall e ranV, NatMap.find e V = Some ranV ->
   (forall e' ranV', e <> e' -> NatMap.find e' V = Some ranV' ->
    (forall c, In c ranV -> ~In c ranV') /\ (forall c, In c ranV' -> ~In c ranV)).
 
+Lemma disjoint_VPT_remove : forall r V,
+  disjoint_VPT V -> disjoint_VPT (NatMap.remove r V).
+Proof.
+  intros.
+  unfold disjoint_VPT in *; intros.
+  assert (NatMap.find (elt:=remapping_list) r (NatMap.remove r V) = None).
+  apply NatMapFacts.remove_eq_o; reflexivity.
+  case_eq (eqb e r); intros.
+  apply cmp_to_eq in H4; subst.
+  rewrite -> H0 in H3; discriminate.
+  case_eq (eqb e' r); intros.
+  apply cmp_to_eq in H5; subst.
+  rewrite -> H2 in H3; discriminate.
+  apply cmp_to_uneq in H4, H5.
+  assert (NatMap.find (elt:=remapping_list) e (NatMap.remove r V) = NatMap.find e V).
+  apply NatMapFacts.remove_neq_o; apply not_eq_sym; exact H4.
+  assert (NatMap.find (elt:=remapping_list) e' (NatMap.remove r V) = NatMap.find e' V).
+  apply NatMapFacts.remove_neq_o; apply not_eq_sym; exact H5.
+  rewrite -> H0 in H6; rewrite -> H2 in H7; apply eq_sym in H6, H7.
+  specialize (H e ranV H6 e' ranV' H1 H7).
+  exact H.
+Qed.
+
+Lemma disjoint_VPT_add : forall r V q l,
+  NatMap.find r V = Some (q :: l) ->
+  disjoint_VPT V -> disjoint_VPT (NatMap.add r l V).
+Proof.
+  intros.
+  unfold disjoint_VPT in *; intros.
+  case_eq (eqb e r); case_eq (eqb e' r); intros.
+  apply cmp_to_eq in H4, H5; subst.
+  unfold not in H2; destruct H2; reflexivity.
+  apply cmp_to_uneq in H4; apply cmp_to_eq in H5; subst.
+  assert (NatMap.find (elt:=remapping_list) r (NatMap.add r l V) = Some l).
+  apply NatMapFacts.add_eq_o; reflexivity.
+  assert (NatMap.find (elt:=remapping_list) e' (NatMap.add r l V)
+  = NatMap.find (elt:=remapping_list) e' V).
+  apply NatMapFacts.add_neq_o; exact H2.
+  rewrite -> H1 in H5; injection H5; intros; subst.
+  rewrite -> H3 in H6; apply eq_sym in H6.
+  specialize (H0 r (q :: l) H e' ranV' H2 H6); destruct H0.
+  split; intros.
+  apply (in_cons q c l) in H8. apply H0 in H8. exact H8.
+  apply H7 in H8. intros contra. apply (in_cons q c l) in contra.
+  apply H8 in contra. exact contra.
+  apply cmp_to_uneq in H5; apply cmp_to_eq in H4; subst.
+  assert (NatMap.find (elt:=remapping_list) r (NatMap.add r l V) = Some l).
+  apply NatMapFacts.add_eq_o; reflexivity.
+  assert (NatMap.find (elt:=remapping_list) e (NatMap.add r l V)
+  = NatMap.find (elt:=remapping_list) e V).
+  apply NatMapFacts.add_neq_o; apply not_eq_sym; exact H2.
+  rewrite -> H3 in H4; injection H4; intros; subst.
+  rewrite -> H1 in H6; apply eq_sym in H6.
+  specialize (H0 e ranV H6 r (q :: l) H2 H); destruct H0.
+  split; intros.
+  apply H0 in H8. intros contra. apply (in_cons q c l) in contra.
+  apply H8 in contra. exact contra.
+  apply (in_cons q c l) in H8. apply H7 in H8. exact H8.
+  apply cmp_to_uneq in H4, H5.
+  assert (NatMap.find (elt:=remapping_list) e (NatMap.add r l V)
+  = NatMap.find (elt:=remapping_list) e V).
+  apply NatMapFacts.add_neq_o; apply not_eq_sym; exact H5.
+  assert (NatMap.find (elt:=remapping_list) e' (NatMap.add r l V)
+  = NatMap.find (elt:=remapping_list) e' V).
+  apply NatMapFacts.add_neq_o; apply not_eq_sym; exact H4.
+  rewrite -> H1 in H6; rewrite -> H3 in H7; apply eq_sym in H6, H7.
+  apply (H0 e ranV H6 e' ranV' H2 H7).
+Qed.
+
+Lemma disjoint_VPT_add2 : forall r V q l,
+  NatMap.find r V = Some l ->
+  (forall e l', NatMap.find e V = Some l' -> ~In q l') ->
+  disjoint_VPT V -> disjoint_VPT (NatMap.add r (q :: l) V).
+Proof.
+  intros.
+  unfold disjoint_VPT in *; intros.
+  case_eq (eqb e r); case_eq (eqb e' r); intros.
+  apply cmp_to_eq in H5, H6; subst.
+  assert (r = r). reflexivity. apply H3 in H5. destruct H5.
+  apply cmp_to_eq in H6. apply cmp_to_uneq in H5. subst e.
+  assert (Some ranV = Some (q :: l)).
+  rewrite <- H2. apply NatMapFacts.add_eq_o; reflexivity.
+  injection H6; intros; subst.
+  assert (NatMap.find (elt:=remapping_list) e' V = Some ranV').
+  apply eq_sym. rewrite <- H4. apply NatMapFacts.add_neq_o; exact H3.
+  split; intros. intros contra. apply in_inv in H8. destruct H8. subst.
+  specialize (H0 e' ranV' H7). apply H0 in contra. exact contra.
+  specialize (H1 r l H e' ranV' H3 H7). destruct H1. apply H1 in H8.
+  apply H8 in contra. exact contra.
+  intros contra. apply in_inv in contra. destruct contra. subst.
+  specialize (H0 e' ranV' H7). apply H0 in H8. exact H8.
+  specialize (H1 r l H e' ranV' H3 H7). destruct H1. apply H1 in H9.
+  apply H9 in H8. exact H8.
+  apply cmp_to_uneq in H6. apply cmp_to_eq in H5. subst e'.
+  assert (Some ranV' = Some (q :: l)).
+  rewrite <- H4. apply NatMapFacts.add_eq_o; reflexivity.
+  injection H5; intros; subst.
+  assert (NatMap.find (elt:=remapping_list) e V = Some ranV).
+  apply eq_sym. rewrite <- H2. apply NatMapFacts.add_neq_o; apply not_eq_sym; exact H3.
+  split; intros. intros contra. apply in_inv in contra. destruct contra. subst.
+  specialize (H0 e ranV H7). apply H0 in H8. exact H8.
+  specialize (H1 e ranV H7 r l H3 H). destruct H1. apply H1 in H8.
+  apply H8 in H9. exact H9.
+  intros contra. apply in_inv in H8. destruct H8. subst.
+  specialize (H0 e ranV H7). apply H0 in contra. exact contra.
+  specialize (H1 e ranV H7 r l H3 H). destruct H1. apply H9 in H8.
+  apply H8 in contra. exact contra.
+  apply cmp_to_uneq in H5, H6.
+  assert (NatMap.find e V = Some ranV). apply eq_sym.
+  rewrite <- H2. apply NatMapFacts.add_neq_o; apply not_eq_sym; exact H6.
+  assert (NatMap.find e' V = Some ranV'). apply eq_sym.
+  rewrite <- H4. apply NatMapFacts.add_neq_o; apply not_eq_sym; exact H5.
+  specialize (H1 e ranV H7 e' ranV' H3 H8). destruct H1.
+  split; intros.
+  apply H1. exact H10.
+  apply H9. exact H10.
+Qed.
+
+(* Well-Formed 3 *)
 Definition wf3 (sigma: runtime_state): Prop :=
   forall k mu rho pi lambda F V C R e ranV,
   (sigma = runtime_state_value k mu rho pi) ->
@@ -205,6 +325,416 @@ Proof.
 Qed.
 
 (* WF3 MLC Allocation *)
+Lemma NoDup_append : forall l l' (c : cachelet_index),
+  NoDup(l) /\ NoDup(l') -> l = c :: nil -> ~In c l' -> NoDup(l ++ l').
+Proof.
+  intros.
+  destruct H.
+  rewrite -> H0.
+  constructor. exact H1. exact H2.
+Qed.
+
+Lemma NoDup_remove : forall c F,
+  NoDup(F) -> NoDup(remove eq_dec_cachelet c F).
+Proof.
+  intros.
+  induction F.
+  assert (~In c nil). unfold In; unfold not; auto.
+  apply (notin_remove eq_dec_cachelet nil c) in H0.
+  rewrite -> H0. exact H.
+  apply NoDup_cons_iff in H. destruct H.
+  unfold remove. case_eq (eq_dec_cachelet c a). intros.
+  apply IHF. exact H0.
+  intros. constructor. intros contra. apply H.
+  assert (In a F /\ a <> c -> In a F). intros. destruct H2. exact H2.
+  apply H2. apply (in_remove eq_dec_cachelet F a c). exact contra.
+  apply IHF. exact H0.
+Qed.
+
+Lemma remove_CAT_not_in : forall c F remF,
+  remove_CAT c F = Some remF -> ~In c remF.
+Proof.
+  intros.
+  unfold remove_CAT in H.
+  destruct (in_bool c F).
+  injection H; intros; subst.
+  apply remove_In. discriminate.
+Qed.
+
+Lemma remove_CAT_in : forall b c F remF,
+  remove_CAT b F = Some remF -> b <> c -> In c F -> In c remF.
+Proof.
+  intros.
+  unfold remove_CAT in H.
+  case_eq (in_bool b F); intros.
+  assert (A0 := H2). destruct (in_bool b F) in A0, H.
+  injection H; intros; subst.
+  apply in_bool_iff in H2. apply in_in_remove.
+  apply not_eq_sym; exact H0. exact H1.
+  discriminate.
+  assert (A0 := H2).
+  destruct (in_bool b F) in A0, H; discriminate.
+Qed.
+
+Lemma remove_CAT_inv_subset : forall w s w0 s0 F remF,
+  remove_CAT (w, s) F = Some remF ->
+  w0 <> w \/ s0 <> s ->
+  ~In (w0, s0) F -> ~In (w0, s0) remF.
+Proof.
+  intros. unfold remove_CAT in H.
+  destruct (in_bool (w, s) F).
+  injection H; intros; subst.
+  intros contra. apply in_remove in contra.
+  destruct contra. apply H1 in H2. exact H2.
+  discriminate.
+Qed.
+
+Lemma wf3_cachelet_allocation : forall n r F V C R F' V' C' R' e ranV ranV',
+  cachelet_allocation n r (single_level_cache F V C R) = Some (single_level_cache F' V' C' R') ->
+  NatMap.find e V = Some ranV ->
+  NatMap.find e V' = Some ranV' ->
+  (forall e' l', NatMap.find e' V = Some l' -> ((forall c, In c l' -> ~ In c F) /\ (forall c, In c F -> ~ In c l'))
+  /\ NoDup(F) /\ NoDup(l') /\ disjoint_VPT(V)) ->
+  (forall e' l', NatMap.find e' V' = Some l' -> ((forall c, In c l' -> ~ In c F') /\ (forall c, In c F' -> ~ In c l'))
+  /\ NoDup(F') /\ NoDup(l') /\ disjoint_VPT(V')).
+Proof.
+  intros n r.
+  induction n.
+  {
+    intros.
+    unfold cachelet_allocation in H.
+    unfold recursive_cachelet_allocation in H.
+    injection H; intros; subst F' V' C' R'.
+    specialize (H2 e' l' H3); exact H2.
+  }
+  {
+    intros F V C R F' V' C' R' e ranV ranV' H H0 H1 H2.
+    unfold cachelet_allocation in H.
+    unfold recursive_cachelet_allocation in H.
+    fold recursive_cachelet_allocation in H.
+    case_eq (way_first_allocation F). intros c H3.
+    assert (A0 := H3). destruct (way_first_allocation F) in H, A0.
+    destruct c0.
+    case_eq (NatMap.find s R). intros p H4.
+    assert (A1 := H4). destruct (NatMap.find s R) in H, A1.
+    case_eq (NatMap.find r V). intros r0 H5.
+    assert (A2 := H5). destruct (NatMap.find r V) in H, A2.
+    case_eq (remove_CAT (w, s) F). intros c0 F0.
+    assert (A3 := F0). destruct (remove_CAT (w, s) F) in H, A3.
+    injection A0; injection A1; injection A2; injection A3;
+    intros X0 X1 X2 X3; subst; clear A0 A1 A2.
+    case_eq (eqb r e); intros V0.
+    {
+      apply cmp_to_eq in V0; subst e.
+      apply (IHn c0 (NatMap.add r ((w, s) :: r0) V) C
+      (NatMap.add s (update p w (enclave_ID_active r)) R) F' V' C' R' r ((w, s) :: r0) ranV').
+      unfold cachelet_allocation; exact H.
+      apply NatMapFacts.add_eq_o; reflexivity. exact H1.
+      intros; case_eq (eqb e' r); intros V0.
+      {
+        apply cmp_to_eq in V0; subst e'.
+        assert (NatMap.find (elt:=remapping_list) r (NatMap.add r ((w, s) :: r0) V)
+        = Some ((w, s) :: r0)).
+        apply NatMapFacts.add_eq_o;  reflexivity.
+        rewrite -> H6 in H7; injection H7; intros; subst. assert (FV := H2).
+        specialize (H2 r ranV H0); destruct H2; destruct H2; destruct H8; destruct H10.
+        assert (DJV := H11); unfold disjoint_VPT in H11.
+        rewrite -> H0 in H5. injection H5; intros; subst.
+        split; split. intros. intros contra.
+        apply in_inv in H12; destruct H12. subst.
+        apply remove_CAT_not_in in F0. apply F0 in contra. exact contra.
+        apply (remove_CAT_f c (w, s) F c0) in contra.
+        apply H9 in contra. apply contra in H12. destruct H12. exact F0.
+        intros; intros contra. apply in_inv in contra. destruct contra. subst.
+        apply (remove_CAT_not_in (w, s) F c0) in F0. apply F0 in H12. exact H12.
+        intros. apply (remove_CAT_f c (w, s) F c0) in H12. apply H9 in H12.
+        apply H12 in H13. exact H13. exact F0.
+        unfold remove_CAT in F0. destruct (in_bool (w, s) F).
+        injection F0; intros; subst. apply NoDup_remove. exact H8.
+        discriminate.
+        split. constructor. intros contra. unfold remove_CAT in F0.
+        case_eq (in_bool (w, s) F). intros. assert (A0 := H12).
+        destruct (in_bool (w, s) F) in A0, H. apply in_bool_iff in H12.
+        apply H9 in H12. apply H12 in contra. exact contra.
+        discriminate.
+        intros; destruct (in_bool (w, s) F); discriminate. exact H10.
+        apply (disjoint_VPT_add2 r V (w, s) r0). exact H0.
+        intros. specialize (FV e l' H12). destruct FV. destruct H13.
+        apply H15. unfold remove_CAT in F0. case_eq (in_bool (w, s) F); intros.
+        assert (A0 := H16). destruct (in_bool (w, s) F) in F0, A0.
+        apply in_bool_iff in H16. exact H16.
+        discriminate.
+        intros; destruct (in_bool (w, s) F); discriminate. exact DJV.
+      }
+      {
+        apply cmp_to_uneq in V0.
+        assert (NatMap.find e' V = Some l').
+        rewrite <- H6. apply eq_sym. apply NatMapFacts.add_neq_o; apply not_eq_sym; exact V0.
+        specialize (H2 e' l' H7) as FV.
+        destruct FV; destruct H8; destruct H9; destruct H11.
+        assert (DJV := H12); unfold disjoint_VPT in H12.
+        split; split. intros.
+        case_eq (eq_cachelet_index c (w, s)); intros;
+        unfold eq_cachelet_index in H14; destruct c.
+        apply cmp_to_eq_and in H14; destruct H14; subst w0 s0.
+        apply (remove_CAT_not_in (w, s) F c0). exact F0.
+        apply cmp_to_uneq_and in H14.
+        apply H8 in H13. 
+        apply (remove_CAT_inv_subset w s w0 s0 F c0).
+        exact F0. exact H14. exact H13.
+        intros; intros contra. apply H8 in contra.
+        apply (remove_CAT_f c (w, s) F c0) in F0. apply contra in F0.
+        exact F0. exact H13.
+        unfold remove_CAT in F0. destruct (in_bool (w, s) F).
+        injection F0; intros; subst.
+        apply NoDup_remove. exact H9. discriminate.
+        split. exact H11.
+        apply (disjoint_VPT_add2 r V (w, s) r0). exact H5.
+        intros. specialize (H2 e l'0 H13). destruct H2. destruct H2.
+        apply H15. unfold remove_CAT in F0. case_eq (in_bool (w, s) F); intros.
+        assert (A0 := H16). destruct (in_bool (w, s) F) in F0, A0.
+        apply in_bool_iff in H16. exact H16.
+        discriminate.
+        intros; destruct (in_bool (w, s) F); discriminate. exact DJV.
+      }
+    }
+    {
+      apply cmp_to_uneq in V0.
+      apply (IHn c0 (NatMap.add r ((w, s) :: r0) V) C
+      (NatMap.add s (update p w (enclave_ID_active r)) R) F' V' C' R' e ranV ranV').
+      unfold cachelet_allocation; exact H.
+      rewrite <- H0. apply NatMapFacts.add_neq_o; exact V0. exact H1.
+      intros; case_eq (eqb e' r); intros V1.
+      {
+        apply cmp_to_eq in V1; subst e'.
+        assert (Some l' = Some ((w, s) :: r0)).
+        rewrite <- H6. apply NatMapFacts.add_eq_o; reflexivity.
+        injection H7; intros; subst.
+        assert (V2 := H2). specialize (H2 r r0 H5).
+        destruct H2; destruct H2; destruct H8; destruct H10.
+        assert (DJV := H11); unfold disjoint_VPT in H11.
+        split; split. intros.
+        apply in_inv in H12. destruct H12. subst.
+        apply (remove_CAT_not_in (w, s) F c0). exact F0.
+        intros contra. apply (remove_CAT_f c (w, s) F c0) in contra.
+        apply H9 in contra. apply contra in H12. exact H12. exact F0.
+        intros. intros contra. apply in_inv in contra. destruct contra. subst.
+        apply (remove_CAT_not_in (w, s) F c0) in F0. apply F0 in H12. exact H12.
+        apply (remove_CAT_f c (w, s) F c0) in H12. apply H9 in H12.
+        apply H12 in H13. exact H13. exact F0.
+        unfold remove_CAT in F0. destruct (in_bool (w, s) F).
+        injection F0; intros; subst.
+        apply NoDup_remove. exact H8. discriminate.
+        split. constructor.
+        apply H9. unfold remove_CAT in F0.
+        case_eq (in_bool (w, s) F); intros.
+        apply in_bool_iff; exact H12.
+        destruct (in_bool (w, s) F); discriminate. exact H10.
+        apply (disjoint_VPT_add2 r V (w, s) r0). exact H5.
+        intros. specialize (V2 e0 l' H12). destruct V2. destruct H13.
+        apply H15. unfold remove_CAT in F0. case_eq (in_bool (w, s) F); intros.
+        assert (A0 := H16). destruct (in_bool (w, s) F) in F0, A0.
+        apply in_bool_iff in H16. exact H16.
+        discriminate.
+        intros; destruct (in_bool (w, s) F); discriminate. exact DJV.
+      }
+      {
+        apply cmp_to_uneq in V1.
+        assert (NatMap.find e' V = Some l').
+        apply eq_sym; rewrite <- H6; apply NatMapFacts.add_neq_o; apply not_eq_sym; exact V1.
+        specialize (H2 e' l' H7) as FV.
+        destruct FV; destruct H8; destruct H9; destruct H11.
+        assert (DJV := H12); unfold disjoint_VPT in H12.
+        split; split. intros. intros contra.
+        apply (remove_CAT_f c (w, s) F c0) in contra.
+        apply H10 in contra. apply contra in H13. exact H13. exact F0.
+        intros. apply H10. apply (remove_CAT_f c (w, s) F c0).
+        exact F0. exact H13.
+        unfold remove_CAT in F0. destruct (in_bool (w, s) F).
+        injection F0; intros; subst.
+        apply NoDup_remove. exact H9. discriminate.
+        split. exact H11.
+        apply (disjoint_VPT_add2 r V (w, s) r0). exact H5.
+        intros. specialize (H2 e0 l'0 H13). destruct H2. destruct H2.
+        apply H15. unfold remove_CAT in F0. case_eq (in_bool (w, s) F); intros.
+        assert (A0 := H16). destruct (in_bool (w, s) F) in F0, A0.
+        apply in_bool_iff in H16. exact H16.
+        discriminate.
+        intros; destruct (in_bool (w, s) F); discriminate. exact DJV.
+      }
+    }
+    discriminate.
+    intros; destruct (remove_CAT (w, s) F).
+    discriminate.
+    discriminate.
+    discriminate.
+    intros; destruct (NatMap.find r V).
+    discriminate.
+    discriminate.
+    discriminate.
+    intros; destruct (NatMap.find s R).
+    discriminate.
+    discriminate.
+    discriminate.
+    intros; destruct (way_first_allocation F).
+    discriminate.
+    discriminate.
+  }
+Qed.
+
+Lemma wf3_mlc_alloc : forall lambda h_tree n state k k' index psi psi' F V C R F' V' C' R' enc ranV ranV',
+  well_defined_cache_tree h_tree ->
+  mlc_allocation n state k lambda h_tree = Some k' ->
+  NatMap.find index k = Some psi ->
+  NatMap.find index k' = Some psi' ->
+  psi = single_level_cache F V C R ->
+  psi' = single_level_cache F' V' C' R' ->
+  NatMap.find (elt:=remapping_list) enc V = Some ranV ->
+  NatMap.find (elt:=remapping_list) enc V' = Some ranV' ->
+  (forall e l, NatMap.find e V = Some l -> ((forall c, In c l -> ~In c F) /\ (forall c, In c F -> ~In c l)) /\ NoDup(F) /\ NoDup(l) /\ disjoint_VPT(V)) ->
+  ((forall c, In c ranV' -> ~In c F') /\ (forall c, In c F' -> ~In c ranV')) /\ NoDup(F') /\ NoDup(ranV') /\ disjoint_VPT(V').
+Proof.
+  unfold mlc_allocation.
+  intros lambda h_tree.
+  case_eq (get_cache_ID_path lambda h_tree).
+  intros l.
+  generalize dependent lambda.
+  induction l.
+  {
+    intros lambda IHTREE n state k k' index psi psi' F V C R
+    F' V' C' R' enc ranV ranV' WFH; intros.
+    destruct state; destruct e.
+    unfold recursive_mlc_deallocation in H.
+    injection H; intros; subst k'.
+    rewrite -> H0 in H1.
+    injection H1; intros; subst psi psi'.
+    injection H7; intros; subst F' V' C' R'.
+    rewrite -> H5 in H4; injection H4; intros; subst.
+    apply (H6 enc ranV). exact H5.
+    discriminate.
+  }
+  {
+    intros lambda IHTREE n state k k' index psi psi' F V C R
+    F' V' C' R' enc ranV ranV' WFH; intros.
+    destruct state; destruct e.
+    unfold recursive_mlc_allocation in H.
+    fold recursive_mlc_allocation in H.
+    destruct n. discriminate.
+    case_eq (NatMap.find a k). intros.
+    assert (A0 := H7). destruct (NatMap.find a k) in A0, H.
+    case_eq (cachelet_allocation n r s0). intros.
+    assert (A1 := H8). destruct (cachelet_allocation n r s0) in A1, H.
+    injection A0; injection A1; intros; subst s0 s2; clear A0 A1.
+    assert (WFH1 := WFH).
+    unfold well_defined_cache_tree in WFH1.
+    destruct WFH1 as [ WFH1 WFH2 ]. destruct WFH2 as [ WFH2 WFH3 ]. destruct WFH3 as [ WFH3 WFH4 ].
+    case_eq (eqb index a).
+    {
+      intros; apply cmp_to_eq in H9; subst a.
+      rewrite -> H7 in H0.
+      injection H0; intros; subst s.
+      destruct s1.
+      case_eq (NatMap.find enc v). intros.
+      destruct l.
+      {
+        apply (IHl root_node WFH1 n0 (enclave_state_value (enclave_ID_active r) (NatMap.empty enclave_memory_range_value))
+        (NatMap.add index (single_level_cache c v w s) k) k' index (single_level_cache c v w s) psi' c v w s F' V' C' R' enc r0 ranV').
+        exact WFH.
+        exact H.
+        apply NatMapFacts.add_eq_o. reflexivity.
+        exact H1.
+        reflexivity.
+        exact H3.
+        exact H9.
+        exact H5.
+        subst psi. apply (wf3_cachelet_allocation n r F V C R c v w s enc ranV r0).
+        exact H8. exact H4. exact H9. exact H6.
+      }
+      {
+        destruct lambda.
+        rewrite -> WFH1 in IHTREE. discriminate.
+        specialize (WFH3 c0 index (p :: l) IHTREE).
+        unfold get_cache_ID_path in IHTREE. discriminate.
+        specialize (WFH2 p0 index (p :: l) IHTREE).
+        injection WFH2; intros; subst p0.
+        apply (WFH4 index p l) in IHTREE.
+        apply (IHl (cache_node p) IHTREE n0 (enclave_state_value (enclave_ID_active r) (NatMap.empty enclave_memory_range_value))
+        (NatMap.add index (single_level_cache c v w s) k) k' index (single_level_cache c v w s) psi' c v w s F' V' C' R' enc r0 ranV').
+        exact WFH.
+        exact H.
+        apply NatMapFacts.add_eq_o. reflexivity.
+        exact H1.
+        reflexivity.
+        exact H3.
+        exact H9.
+        exact H5.
+        subst psi. apply (wf3_cachelet_allocation n r F V C R c v w s enc ranV r0).
+        exact H8. exact H4. exact H9. exact H6.
+      }
+      {
+        intros. destruct psi.
+        injection H2; intros; subst c0 v0 w0 s0.
+        apply (cachelet_allocation_v n r F V C R c v w s enc) in H8.
+        assert (NatMap.find enc V <> None).
+        intros contra; rewrite -> contra in H4; discriminate.
+        apply NatMapFacts.in_find_iff in H10.
+        apply NatMapFacts.not_find_in_iff in H9.
+        apply H8 in H10. apply H9 in H10. destruct H10.
+      }
+    }
+    {
+      intros; apply cmp_to_uneq in H9.
+      destruct l.
+      {
+        apply (IHl root_node WFH1 n0 (enclave_state_value (enclave_ID_active r) (NatMap.empty enclave_memory_range_value))
+        (NatMap.add a s1 k) k' index psi psi' F V C R F' V' C' R' enc ranV ranV').
+        exact WFH.
+        unfold mlc_allocation. exact H.
+        rewrite <- H0. apply NatMapFacts.add_neq_o.
+        apply not_eq_sym. exact H9.
+        exact H1.
+        exact H2.
+        exact H3.
+        exact H4.
+        exact H5.
+        exact H6.
+      }
+      {
+        destruct lambda.
+        rewrite -> WFH1 in IHTREE. discriminate.
+        specialize (WFH3 c a (p :: l) IHTREE).
+        unfold get_cache_ID_path in IHTREE. discriminate.
+        specialize (WFH2 p0 a (p :: l) IHTREE).
+        injection WFH2; intros; subst p0.
+        apply (WFH4 a p l) in IHTREE.
+        apply (IHl (cache_node p) IHTREE n0 (enclave_state_value (enclave_ID_active r) (NatMap.empty enclave_memory_range_value))
+        (NatMap.add a s1 k) k' index psi psi' F V C R F' V' C' R' enc ranV ranV').
+        exact WFH.
+        unfold mlc_allocation. exact H.
+        rewrite <- H0. apply NatMapFacts.add_neq_o.
+        apply not_eq_sym. exact H9.
+        exact H1.
+        exact H2.
+        exact H3.
+        exact H4.
+        exact H5.
+        exact H6.
+      }
+    }
+    discriminate.
+    intros; destruct (cachelet_allocation n r s0).
+    discriminate.
+    discriminate.
+    discriminate.
+    intros; destruct (NatMap.find a k).
+    discriminate.
+    discriminate.
+    discriminate.
+  }
+  intros; destruct (get_cache_ID_path lambda h_tree).
+  discriminate.
+  destruct state; destruct e; discriminate.
+Qed.
 
 (* WF3 MLC Write *)
 Lemma wf3_mlc_write : forall lambda h_tree k e' m0 l0 v D obs1 mu k' index psi psi'
@@ -387,123 +917,6 @@ Proof.
 Qed.
 
 (* WF3 MLC Deallocation *)
-Lemma wf3_clear_remapping_list : forall r ranV F V C R F' V' C' R' ranV',
-  clear_remapping_list r ranV F V C R = Some (single_level_cache F' V' C' R') ->
-  NatMap.find r V = Some ranV ->
-  NatMap.find r V' = Some ranV' ->
-  ((forall c, In c ranV -> ~ In c F) /\ (forall c, In c F -> ~ In c ranV)) /\ NoDup(F) /\ NoDup(ranV) /\ disjoint_VPT(V)  ->
-  ((forall c, In c ranV' -> ~ In c F') /\ (forall c, In c F' -> ~ In c ranV')) /\ NoDup(F') /\ NoDup(ranV') /\ disjoint_VPT(V') .
-Proof.
-  intros r l.
-  induction l.
-  {
-    intros.
-    unfold clear_remapping_list in H.
-    injection H; intros; subst.
-    assert (NatMap.find r (NatMap.remove r V) = None).
-    apply NatMapFacts.remove_eq_o; reflexivity.
-    rewrite -> H3 in H1. discriminate.
-  }
-  {
-    intros.
-    unfold clear_remapping_list in H.
-    fold clear_remapping_list in H.
-    destruct a.
-    case_eq (NatMap.find s R). intros.
-    assert (A0 := H3). destruct (NatMap.find s R) in A0, H.
-    case_eq (cachelet_invalidation C (w, s)). intros.
-    assert (A1 := H4). destruct (cachelet_invalidation C (w, s)) in A1, H.
-    injection A0; injection A1; intros; subst w1 p; clear A0 A1.
-    apply (IHl ((w, s) :: F) (NatMap.add r l V) w0 (NatMap.add s (update p0 w
-    (enclave_ID_active r)) R) F' V' C' R' ranV').
-    exact H.
-    apply NatMapFacts.add_eq_o; reflexivity.
-    exact H1.
-    {
-      destruct H2; destruct H2; destruct H5; destruct H7.
-      split; split.
-      intros. intros contra.
-      apply in_inv in contra. destruct contra.
-      subst c.
-      apply NoDup_cons_iff in H7. destruct H7.
-      apply H7 in H9. exact H9.
-      apply H6 in H10.
-      assert (In c ((w, s) :: l)).
-      apply in_cons; exact H9.
-      apply H10 in H11. exact H11.
-      intros. intros contra.
-      apply in_inv in H9. destruct H9.
-      subst c.
-      apply NoDup_cons_iff in H7. destruct H7.
-      apply H7 in contra. exact contra.
-      apply H6 in H9.
-      assert (In c ((w, s) :: l)).
-      apply in_cons; exact contra.
-      apply H9 in H10. exact H10.
-      constructor.
-      apply NoDup_cons_iff in H7. destruct H7.
-      intros contra.
-      apply H6 in contra.
-      unfold not in contra.
-      assert (In (w, s) ((w, s) :: l)).
-      apply in_eq; reflexivity.
-      apply contra in H10. exact H10.
-      exact H5. split.
-      apply NoDup_cons_iff in H7. destruct H7. exact H9.
-      {
-        unfold disjoint_VPT in *.
-        intros e ranV H9 e' ranV'0 H10 H11.
-        case_eq (eqb e r); case_eq (eqb e' r); intros.
-        apply cmp_to_eq in H12, H13; subst.
-        unfold not in H10; destruct H10; reflexivity.
-        apply cmp_to_uneq in H12; apply cmp_to_eq in H13; subst.
-        assert (NatMap.find (elt:=remapping_list) r (NatMap.add r l V) = Some l).
-        apply NatMapFacts.add_eq_o; reflexivity.
-        rewrite -> H9 in H13; injection H13; intros; subst.
-        assert (NatMap.find (elt:=remapping_list) e' (NatMap.add r l V) = NatMap.find e' V).
-        apply NatMapFacts.add_neq_o; exact H10.
-        rewrite -> H11 in H14; apply eq_sym in H14.
-        specialize (H8 r ((w, s) :: l) H0 e' ranV'0 H10 H14); destruct H8.
-        split; intros.
-        intros contra. apply H15 in contra.
-        apply (in_cons (w, s) c l) in H16.
-        apply contra in H16. destruct H16.
-        intros contra. apply (in_cons (w, s) c l) in contra.
-        apply H8 in contra. apply contra in H16. destruct H16.
-        apply cmp_to_eq in H12; apply cmp_to_uneq in H13; subst.
-        assert (NatMap.find (elt:=remapping_list) e (NatMap.add r l V) = NatMap.find e V).
-        apply NatMapFacts.add_neq_o; apply not_eq_sym; exact H10.
-        rewrite -> H9 in H12; apply eq_sym in H12.
-        assert (NatMap.find (elt:=remapping_list) r (NatMap.add r l V) = Some l).
-        apply NatMapFacts.add_eq_o; reflexivity.
-        rewrite -> H11 in H14; injection H14; intros; subst.
-        specialize (H8 e ranV H12 r ((w, s) :: l) H10 H0); destruct H8.
-        split; intros.
-        intros contra. apply (in_cons (w, s) c l) in contra.
-        apply H15 in contra. apply contra in H16. destruct H16.
-        intros contra. apply H8 in contra.
-        apply (in_cons (w, s) c l) in H16.
-        apply contra in H16. destruct H16.
-        apply cmp_to_uneq in H12, H13.
-        assert (NatMap.find (elt:=remapping_list) e (NatMap.add r l V) = NatMap.find e V).
-        apply NatMapFacts.add_neq_o; apply not_eq_sym; exact H13.
-        assert (NatMap.find (elt:=remapping_list) e' (NatMap.add r l V) = NatMap.find e' V).
-        apply NatMapFacts.add_neq_o; apply not_eq_sym; exact H12.
-        rewrite -> H9 in H14. rewrite -> H11 in H15. apply eq_sym in H14, H15.
-        specialize (H8 e ranV H14 e' ranV'0 H10 H15); exact H8.
-      }
-    }
-    discriminate.
-    intros; destruct (cachelet_invalidation C (w, s)).
-    discriminate.
-    discriminate.
-    discriminate.
-    intros; destruct (NatMap.find s R).
-    discriminate.
-    discriminate.
-  }
-Qed.
-
 Lemma clear_remapping_list_ranV : forall r l F V C R F' V' C' R' e ranV ranV',
   r <> e -> clear_remapping_list r l F V C R = Some (single_level_cache F' V' C' R') ->
   NatMap.find e V = Some ranV ->
@@ -539,171 +952,7 @@ Proof.
   }
 Qed.
 
-Lemma disjoint_VPT_remove : forall r V,
-  disjoint_VPT V -> disjoint_VPT (NatMap.remove r V).
-Proof.
-  intros.
-  unfold disjoint_VPT in *; intros.
-  assert (NatMap.find (elt:=remapping_list) r (NatMap.remove r V) = None).
-  apply NatMapFacts.remove_eq_o; reflexivity.
-  case_eq (eqb e r); intros.
-  apply cmp_to_eq in H4; subst.
-  rewrite -> H0 in H3; discriminate.
-  case_eq (eqb e' r); intros.
-  apply cmp_to_eq in H5; subst.
-  rewrite -> H2 in H3; discriminate.
-  apply cmp_to_uneq in H4, H5.
-  assert (NatMap.find (elt:=remapping_list) e (NatMap.remove r V) = NatMap.find e V).
-  apply NatMapFacts.remove_neq_o; apply not_eq_sym; exact H4.
-  assert (NatMap.find (elt:=remapping_list) e' (NatMap.remove r V) = NatMap.find e' V).
-  apply NatMapFacts.remove_neq_o; apply not_eq_sym; exact H5.
-  rewrite -> H0 in H6; rewrite -> H2 in H7; apply eq_sym in H6, H7.
-  specialize (H e ranV H6 e' ranV' H1 H7).
-  exact H.
-Qed.
-
-Lemma disjoint_VPT_add : forall r V q l,
-  NatMap.find r V = Some (q :: l) ->
-  disjoint_VPT V -> disjoint_VPT (NatMap.add r l V).
-Proof.
-  intros.
-  unfold disjoint_VPT in *; intros.
-  case_eq (eqb e r); case_eq (eqb e' r); intros.
-  apply cmp_to_eq in H4, H5; subst.
-  unfold not in H2; destruct H2; reflexivity.
-  apply cmp_to_uneq in H4; apply cmp_to_eq in H5; subst.
-  assert (NatMap.find (elt:=remapping_list) r (NatMap.add r l V) = Some l).
-  apply NatMapFacts.add_eq_o; reflexivity.
-  assert (NatMap.find (elt:=remapping_list) e' (NatMap.add r l V)
-  = NatMap.find (elt:=remapping_list) e' V).
-  apply NatMapFacts.add_neq_o; exact H2.
-  rewrite -> H1 in H5; injection H5; intros; subst.
-  rewrite -> H3 in H6; apply eq_sym in H6.
-  specialize (H0 r (q :: l) H e' ranV' H2 H6); destruct H0.
-  split; intros.
-  apply (in_cons q c l) in H8. apply H0 in H8. exact H8.
-  apply H7 in H8. intros contra. apply (in_cons q c l) in contra.
-  apply H8 in contra. exact contra.
-  apply cmp_to_uneq in H5; apply cmp_to_eq in H4; subst.
-  assert (NatMap.find (elt:=remapping_list) r (NatMap.add r l V) = Some l).
-  apply NatMapFacts.add_eq_o; reflexivity.
-  assert (NatMap.find (elt:=remapping_list) e (NatMap.add r l V)
-  = NatMap.find (elt:=remapping_list) e V).
-  apply NatMapFacts.add_neq_o; apply not_eq_sym; exact H2.
-  rewrite -> H3 in H4; injection H4; intros; subst.
-  rewrite -> H1 in H6; apply eq_sym in H6.
-  specialize (H0 e ranV H6 r (q :: l) H2 H); destruct H0.
-  split; intros.
-  apply H0 in H8. intros contra. apply (in_cons q c l) in contra.
-  apply H8 in contra. exact contra.
-  apply (in_cons q c l) in H8. apply H7 in H8. exact H8.
-  apply cmp_to_uneq in H4, H5.
-  assert (NatMap.find (elt:=remapping_list) e (NatMap.add r l V)
-  = NatMap.find (elt:=remapping_list) e V).
-  apply NatMapFacts.add_neq_o; apply not_eq_sym; exact H5.
-  assert (NatMap.find (elt:=remapping_list) e' (NatMap.add r l V)
-  = NatMap.find (elt:=remapping_list) e' V).
-  apply NatMapFacts.add_neq_o; apply not_eq_sym; exact H4.
-  rewrite -> H1 in H6; rewrite -> H3 in H7; apply eq_sym in H6, H7.
-  apply (H0 e ranV H6 e' ranV' H2 H7).
-Qed.
-
-Lemma wf3_clear_remapping_list_uneq : forall r l F V C R F' V' C' R' e ranV ranV',
-  e <> r -> clear_remapping_list r l F V C R = Some (single_level_cache F' V' C' R') ->
-  NatMap.find r V = Some l ->
-  NatMap.find e V = Some ranV ->
-  NatMap.find e V' = Some ranV' ->
-  ((forall c, In c ranV -> ~ In c F) /\ (forall c, In c F -> ~ In c ranV)) /\ NoDup(F) /\ NoDup(ranV) /\ disjoint_VPT(V) ->
-  ((forall c, In c l -> ~ In c F) /\ (forall c, In c F -> ~ In c l)) /\ NoDup(l) ->
-  ((forall c, In c ranV' -> ~ In c F') /\ (forall c, In c F' -> ~ In c ranV')) /\ NoDup(F') /\ NoDup(ranV') /\ disjoint_VPT(V').
-Proof.
-  intros r l.
-  induction l.
-  {
-    intros.
-    unfold clear_remapping_list in H0.
-    injection H0; intros; subst.
-    assert (NatMap.find e (NatMap.remove r V) = NatMap.find e V).
-    apply NatMapFacts.remove_neq_o; apply not_eq_sym; exact H.
-    rewrite -> H3 in H6; rewrite -> H2 in H6.
-    injection H6; intros; subst.
-    split; destruct H4. exact H4.
-    split; destruct H7. exact H7.
-    split; destruct H8. exact H8.
-    apply disjoint_VPT_remove; exact H9.
-  }
-  {
-    intros.
-    unfold clear_remapping_list in H0.
-    fold clear_remapping_list in H0.
-    destruct a.
-    case_eq (NatMap.find s R). intros.
-    assert (A0 := H6). destruct (NatMap.find s R) in A0, H0.
-    case_eq (cachelet_invalidation C (w, s)). intros.
-    assert (A1 := H7). destruct (cachelet_invalidation C (w, s)) in A1, H0.
-    injection A0; injection A1; intros; subst w1 p; clear A0 A1.
-    assert (ranV = ranV').
-    apply (clear_remapping_list_ranV r l ((w, s) :: F) (NatMap.add r l V) w0 (NatMap.add s
-    (update p0 w (enclave_ID_active r)) R) F' V' C' R' e ranV ranV').
-    apply not_eq_sym; exact H. exact H0.
-    rewrite <- H2. apply NatMapFacts.add_neq_o. apply not_eq_sym; exact H.
-    exact H3. subst ranV'.
-    apply (IHl ((w, s) :: F) (NatMap.add r l V) w0 (NatMap.add s (update p0 w
-    (enclave_ID_active r)) R) F' V' C' R' e ranV ranV).
-    exact H. exact H0.
-    apply NatMapFacts.add_eq_o; reflexivity.
-    rewrite <- H2. apply NatMapFacts.add_neq_o; apply not_eq_sym; exact H.
-    exact H3.
-    {
-      destruct H4; destruct H4; destruct H8; destruct H10.
-      destruct H5 as [ H5 N ]. destruct H5 as [ H5 H5' ].
-      assert (V0 := H11).
-      unfold disjoint_VPT in H11.
-      specialize (H11 e ranV H2 r ((w, s) :: l) H H1); destruct H11.
-      split; split.
-      intros. intros contra.
-      apply in_inv in contra. destruct contra.
-      subst c. apply H11 in H13.
-      unfold In in H13. destruct H13. left; reflexivity.
-      apply H9 in H14. apply H14 in H13. exact H13.
-      intros. intros contra.
-      apply in_inv in H13. destruct H13.
-      subst c. apply H11 in contra.
-      unfold In in contra. destruct contra. left; reflexivity.
-      apply H9 in H13. apply H13 in contra. exact contra.
-      constructor.
-      assert (In (w, s) ((w, s) :: l)).
-      apply in_eq; reflexivity.
-      apply H5 in H13. exact H13. exact H8.
-      split. exact H10.
-      apply (disjoint_VPT_add r V (w, s) l).
-      exact H1. exact V0.
-    }
-    destruct H5; destruct H5.
-    split. split; intros.
-    intros contra. apply in_inv in contra. destruct contra. subst c.
-    apply NoDup_cons_iff in H8. destruct H8.
-    apply H8 in H10. exact H10.
-    apply (in_cons (w, s) c l) in H10. apply H9 in H11.
-    apply H11 in H10. exact H10.
-    intros contra. apply in_inv in H10. destruct H10. subst c.
-    apply NoDup_cons_iff in H8. destruct H8.
-    apply H8 in contra. exact contra.
-    apply (in_cons (w, s) c l) in contra. apply H9 in H10.
-    apply H10 in contra. exact contra.
-    apply NoDup_cons_iff in H8. destruct H8. exact H10.
-    discriminate.
-    intros; destruct (cachelet_invalidation C (w, s)).
-    discriminate.
-    discriminate.
-    discriminate.
-    intros; destruct (NatMap.find s R).
-    discriminate.
-    discriminate.
-  }
-Qed.
-
-Lemma hard : forall r l F V C R F' V' C' R' e ranV ranV',
+Lemma wf3_clear_remapping_list : forall r l F V C R F' V' C' R' e ranV ranV',
   clear_remapping_list r l F V C R = Some (single_level_cache F' V' C' R') ->
   NatMap.find r V = Some l ->
   NatMap.find e V = Some ranV ->
@@ -719,29 +968,174 @@ Proof.
     intros.
     unfold clear_remapping_list in H.
     injection H; intros; subst.
-    case_eq (eqb e r); intros V0.
+    case_eq (eqb e' r); intros V0.
     {
       apply cmp_to_eq in V0; subst.
       assert (NatMap.find r (NatMap.remove r V) = None).
       apply NatMapFacts.remove_eq_o; reflexivity.
-      rewrite -> H2 in H5. discriminate.
+      rewrite -> H4 in H5. discriminate.
     }
     {
       apply cmp_to_uneq in V0.
-      assert (NatMap.find e (NatMap.remove r V) = NatMap.find e V).
+      assert (NatMap.find (elt:=remapping_list) e' (NatMap.remove r V) = NatMap.find e' V).
       apply NatMapFacts.remove_neq_o; apply not_eq_sym; exact V0.
-      rewrite -> H2 in H5; rewrite -> H1 in H5.
-      injection H5; intros; subst.
-      specialize (H3
-
-(* TODO *)
-
-      split; destruct H4. exact H4.
-      split; destruct H7. exact H7.
-      split; destruct H8. exact H8.
-      apply disjoint_VPT_remove; exact H9.
+      rewrite -> H4 in H5; apply eq_sym in H5.
+      specialize (H3 e' l' H5).
+      destruct H3; split. exact H3.
+      destruct H6; split. exact H6.
+      destruct H7; split. exact H7.
+      apply disjoint_VPT_remove; exact H8.
     }
   }
+  {
+    intros F V C R F' V' C' R' e ranV ranV' H H0 H1 H2 H3.
+    unfold clear_remapping_list in H.
+    fold clear_remapping_list in H.
+    destruct a.
+    case_eq (NatMap.find s R). intros p H4.
+    assert (A0 := H4). destruct (NatMap.find s R) in A0, H.
+    case_eq (cachelet_invalidation C (w, s)). intros w0 H5.
+    assert (A1 := H5). destruct (cachelet_invalidation C (w, s)) in A1, H.
+    injection A0; injection A1; intros X Y; subst w1 p; clear A0 A1.
+    case_eq (eqb e r); intros V0.
+    {
+      apply cmp_to_eq in V0; subst e.
+      apply (IHl ((w, s) :: F) (NatMap.add r l V) w0 (NatMap.add s (update p0 w
+      (enclave_ID_active r)) R) F' V' C' R' r l ranV').
+      exact H.
+      apply NatMapFacts.add_eq_o; reflexivity.
+      apply NatMapFacts.add_eq_o; reflexivity.
+      exact H2.
+      intros.
+      case_eq (eqb e' r); intros.
+      {
+        apply cmp_to_eq in H7; subst e'.
+        assert (NatMap.find (elt:=remapping_list) r (NatMap.add r l V) = Some l).
+        apply NatMapFacts.add_eq_o; reflexivity.
+        rewrite -> H6 in H7; injection H7; intros; subst l'.
+        rewrite -> H0 in H1; injection H1; intros; subst ranV.
+        assert (FV := H3). specialize (H3 r ((w, s) :: l) H0).
+        destruct H3; destruct H3; destruct H8; destruct H10.
+        split; split. intros. intros contra.
+        apply in_inv in contra. destruct contra. subst c.
+        apply NoDup_cons_iff in H10. destruct H10. apply H10 in H12. exact H12.
+        apply H9 in H13. apply (in_cons (w, s) c l) in H12.
+        apply H13 in H12. exact H12.
+        intros. intros contra.
+        apply in_inv in H12. destruct H12. subst c.
+        apply NoDup_cons_iff in H10. destruct H10. apply H10 in contra. exact contra.
+        apply H9 in H12. apply (in_cons (w, s) c l) in contra.
+        apply H12 in contra. exact contra.
+        constructor.
+        specialize (FV r ((w, s) :: l) H0). destruct FV; destruct H12.
+        intros contra. apply H14 in contra.
+        assert (In (w, s) ((w, s) :: l)). apply in_eq; reflexivity.
+        apply contra in H15; exact H15. exact H8.
+        split. apply NoDup_cons_iff in H10; destruct H10; exact H12.
+        apply (disjoint_VPT_add r V (w, s) l). exact H0. exact H11.
+      }
+      {
+        apply cmp_to_uneq in H7.
+        assert (NatMap.find (elt:=remapping_list) e' (NatMap.add r l V) = NatMap.find e' V).
+        apply NatMapFacts.add_neq_o; apply not_eq_sym; exact H7.
+        rewrite -> H8 in H6.
+        rewrite -> H0 in H1; injection H1; intros; subst ranV.
+        assert (FV := H3). specialize (H3 e' l' H6).
+        destruct H3; destruct H3; destruct H9; destruct H11.
+        assert (DJV := H12). unfold disjoint_VPT in H12.
+        split; split. intros. intros contra.
+        apply in_inv in contra. destruct contra. subst c.
+        specialize (H12 e' l' H6 r ((w, s) :: l) H7 H0). destruct H12.
+        apply H12 in H13.
+        assert (In (w, s) ((w, s) :: l)). apply in_eq; reflexivity.
+        apply H13 in H15. exact H15.
+        apply H10 in H14. apply H14 in H13. exact H13.
+        intros. intros contra.
+        apply in_inv in H13. destruct H13. subst c.
+        specialize (H12 e' l' H6 r ((w, s) :: l) H7 H0). destruct H12.
+        apply H12 in contra.
+        assert (In (w, s) ((w, s) :: l)). apply in_eq; reflexivity.
+        apply contra in H14. exact H14.
+        apply H10 in H13. apply H13 in contra. exact contra.
+        constructor.
+        specialize (FV r ((w, s) :: l) H0). destruct FV. destruct H13.
+        apply H13. apply in_eq; reflexivity. exact H9.
+        split. exact H11.
+        apply (disjoint_VPT_add r V (w, s) l). exact H0. exact DJV.
+      }
+    }
+    {
+      apply cmp_to_uneq in V0.
+      apply (IHl ((w, s) :: F) (NatMap.add r l V) w0 (NatMap.add s (update p0 w
+      (enclave_ID_active r)) R) F' V' C' R' e ranV ranV').
+      exact H.
+      apply NatMapFacts.add_eq_o; reflexivity.
+      rewrite <- H1. apply NatMapFacts.add_neq_o; apply not_eq_sym; exact V0.
+      exact H2.
+      intros.
+      case_eq (eqb e' r); intros.
+      {
+        apply cmp_to_eq in H7; subst e'.
+        assert (NatMap.find (elt:=remapping_list) r (NatMap.add r l V) = Some l).
+        apply NatMapFacts.add_eq_o; reflexivity.
+        rewrite -> H6 in H7; injection H7; intros; subst l'.
+        specialize (H3 r ((w, s) :: l) H0).
+        destruct H3; destruct H3; destruct H8; destruct H10.
+        split; split.
+        intros. intros contra.
+        apply in_inv in contra. destruct contra. subst c.
+        apply NoDup_cons_iff in H10. destruct H10. apply H10 in H12.
+        exact H12. apply H9 in H13. apply (in_cons (w, s) c l) in H12.
+        apply H13 in H12. exact H12.
+        intros. intros contra.
+        apply in_inv in H12. destruct H12. subst c.
+        apply NoDup_cons_iff in H10. destruct H10. apply H10 in contra.
+        exact contra. apply H9 in H12. apply (in_cons (w, s) c l) in contra.
+        apply H12 in contra. exact contra.
+        apply NoDup_cons_iff. split. intros contra.
+        assert (In (w, s) ((w, s) :: l)). apply in_eq; reflexivity.
+        apply H3 in H12. apply H12 in contra. exact contra. exact H8.
+        split. apply NoDup_cons_iff in H10. destruct H10. exact H12.
+        apply (disjoint_VPT_add r V (w, s) l). exact H0. exact H11.
+      }
+      {
+        apply cmp_to_uneq in H7.
+        assert (NatMap.find (elt:=remapping_list) e' (NatMap.add r l V) = NatMap.find e' V).
+        apply NatMapFacts.add_neq_o; apply not_eq_sym; exact H7.
+        rewrite -> H8 in H6.
+        assert (FV := H3). specialize (H3 e' l' H6).
+        destruct H3; destruct H3; destruct H9; destruct H11.
+        assert (DJV := H12). unfold disjoint_VPT in H12.
+        split; split. intros. intros contra.
+        apply in_inv in contra. destruct contra. subst c.
+        assert (In (w, s) ((w, s) :: l)).
+        apply in_eq; reflexivity. specialize (H12 e' l' H6 r ((w, s) :: l) H7 H0).
+        destruct H12. apply H12 in H13. apply H13 in H14. exact H14.
+        apply H10 in H14. apply H14 in H13. exact H13.
+        intros. intros contra.
+        apply in_inv in H13. destruct H13. subst c.
+        assert (In (w, s) ((w, s) :: l)).
+        apply in_eq; reflexivity. specialize (H12 e' l' H6 r ((w, s) :: l) H7 H0).
+        destruct H12. apply H12 in H13. exact H13. exact contra.
+        apply H10 in H13. apply H13 in contra. exact contra.
+        constructor.
+        assert (In (w, s) ((w, s) :: l)).
+        apply in_eq; reflexivity.
+        specialize (FV r ((w, s) :: l) H0). destruct FV; destruct H14.
+        apply H14 in H13. exact H13. exact H9. split. exact H11.
+        apply (disjoint_VPT_add r V (w, s) l). exact H0. exact DJV.
+      }
+    }
+    discriminate.
+    intros; destruct (cachelet_invalidation C (w, s)).
+    discriminate.
+    discriminate.
+    discriminate.
+    intros; destruct (NatMap.find s R).
+    discriminate.
+    discriminate.
+  }
+Qed.
 
 Lemma wf3_mlc_dealloc : forall lambda h_tree state k k' index psi psi' F V C R F' V' C' R' enc ranV ranV',
   well_defined_cache_tree h_tree ->
@@ -752,7 +1146,7 @@ Lemma wf3_mlc_dealloc : forall lambda h_tree state k k' index psi psi' F V C R F
   psi' = single_level_cache F' V' C' R' ->
   NatMap.find (elt:=remapping_list) enc V = Some ranV ->
   NatMap.find (elt:=remapping_list) enc V' = Some ranV' ->
-  (forall e l, NatMap.find e V = Some l -> ((forall c, In c ranV -> ~In c F) /\ (forall c, In c F -> ~In c ranV)) /\ NoDup(F) /\ NoDup(ranV) /\ disjoint_VPT(V)) ->
+  (forall e l, NatMap.find e V = Some l -> ((forall c, In c l -> ~In c F) /\ (forall c, In c F -> ~In c l)) /\ NoDup(F) /\ NoDup(l) /\ disjoint_VPT(V)) ->
   ((forall c, In c ranV' -> ~In c F') /\ (forall c, In c F' -> ~In c ranV')) /\ NoDup(F') /\ NoDup(ranV') /\ disjoint_VPT(V').
 Proof.
   unfold mlc_deallocation.
@@ -808,42 +1202,11 @@ Proof.
         exact H9.
         exact H5.
         unfold cachelet_deallocation in H8. destruct psi.
-
-
-
-
-        case_eq (NatMap.find r v0). intros.
+        case_eq (NatMap.find r v0). intros r1 H10.
         assert (A0 := H10). destruct (NatMap.find r v0) in A0, H8.
-        injection A0; injection H2; intros; subst c0 v0 w0 s0 r1; clear A0.
-        case_eq (eqb r enc); intros.
-        apply cmp_to_eq in H11; subst enc.
-        apply (wf3_clear_remapping_list r r2 F V C R c v w s r0) in H8.
-        exact H8. exact H10. exact H9.
-        rewrite -> H4 in H10.
-        injection H10; intros; subst.
-        exact H6.
-        apply cmp_to_uneq in H11.
-        apply (wf3_clear_remapping_list_uneq r r2 F V C R c v w s enc ranV r0).
-        apply not_eq_sym; exact H11. exact H8. exact H10.
-        exact H4. exact H9. exact H6.
-        destruct H6. destruct H12.
-
-
-        assert (H12 := H8).
-        apply (clear_remapping_list_ranV r r2 F V C R c v w s enc ranV r0) in H8.
-        subst r0.
-        destruct H6; destruct H6; destruct H8.
-        split; split.
-        intros. intros contra.
-        apply H6 in H15.
-        assert (In c0 F -> In c0 c).
-        apply (clear_remapping_list_f r r2 F V C R c v w s c0) in H12.
-        intros; exact H12. exact H10.
-        
-
-
-
-
+        injection A0; injection H2; intros X0 X1 X2 X3 X4; subst c0 v0 w0 s0 r1; clear A0.
+        apply (wf3_clear_remapping_list r r2 F V C R c v w s enc ranV r0).
+        exact H8. exact H10. exact H4. exact H9. exact H6.
         discriminate.
         intros; destruct (NatMap.find r v0).
         discriminate.
@@ -852,13 +1215,13 @@ Proof.
       {
         destruct lambda.
         rewrite -> WFH1 in IHTREE. discriminate.
-        specialize (WFH3 c1 index (p :: l) IHTREE).
+        specialize (WFH3 c0 index (p :: l) IHTREE).
         unfold get_cache_ID_path in IHTREE. discriminate.
         specialize (WFH2 p0 index (p :: l) IHTREE).
         injection WFH2; intros; subst p0.
         apply (WFH4 index p l) in IHTREE.
-        apply (IHl (cache_node p) IHTREE (NatMap.add index (single_level_cache c0 v w s) k) k' index
-        (single_level_cache c0 v w s) psi' c0 v w s F' V' C' R' c enc l0 ranV').
+        apply (IHl (cache_node p) IHTREE (NatMap.add index (single_level_cache c v w s) k) k' index
+        (single_level_cache c v w s) psi' c v w s F' V' C' R' enc r0 ranV').
         exact WFH.
         unfold mlc_deallocation. exact H.
         apply NatMapFacts.add_eq_o. reflexivity.
@@ -867,26 +1230,43 @@ Proof.
         exact H3.
         exact H9.
         exact H5.
-        destruct psi.
-        (*
-        apply (wf2_cachelet_deallocation r psi (single_level_cache c0 v w s) F V C R
-        c0 v w s enc ranV l0 c).
-        exact H9. exact H2. reflexivity. exact H4.
-        exact H10. exact H6. exact H7.
-        *)
-        give_up.
+        unfold cachelet_deallocation in H8. destruct psi.
+        case_eq (NatMap.find r v0). intros r1 H10.
+        assert (A0 := H10). destruct (NatMap.find r v0) in A0, H8.
+        injection A0; injection H2; intros X0 X1 X2 X3 X4; subst c0 v0 w0 s0 r1; clear A0.
+        apply (wf3_clear_remapping_list r r2 F V C R c v w s enc ranV r0).
+        exact H8. exact H10. exact H4. exact H9. exact H6.
+        discriminate.
+        intros; destruct (NatMap.find r v0).
+        discriminate.
+        discriminate.
       }
       {
         intros. destruct psi.
-        injection H2; intros; subst c1 v0 w0 s0.
-        apply (cachelet_deallocation_v r (single_level_cache F V C R) (single_level_cache c0 v w s)
-        F V C R c0 v w s enc) in H8.
-        apply V_range_in in H4. apply V_range_not_in in H9.
-        apply H8 in H4.
-        apply H9 in H4.
-        destruct H4.
-        reflexivity.
-        reflexivity.
+        injection H2; intros; subst c0 v0 w0 s0.
+        case_eq (eqb r enc); intros V0.
+        {
+          apply cmp_to_eq in V0; subst enc.
+          apply (wf2_mlc_dealloc_helper r l k k' (NatMap.add index (single_level_cache c v w s) k)
+          index F V C R c v w s F' V' C' R' ranV) in H.
+          rewrite -> H in H5; discriminate.
+          exact H7. subst psi'; exact H1. exact H4. exact H9.
+          apply NatMapFacts.add_eq_o; reflexivity.
+        }
+        {
+          apply (cachelet_deallocation_v r (single_level_cache F V C R) (single_level_cache c v w s)
+          F V C R c v w s enc) in H8.
+          assert (NatMap.find enc V <> None). intros contra.
+          rewrite -> H4 in contra. discriminate.
+          apply NatMapFacts.in_find_iff in H10.
+          apply NatMapFacts.not_find_in_iff in H9.
+          apply H8 in H10.
+          apply H9 in H10.
+          destruct H10.
+          reflexivity.
+          reflexivity.
+          apply cmp_to_uneq in V0; exact V0.
+        }
       }
     }
     {
@@ -894,7 +1274,7 @@ Proof.
       destruct l.
       {
         apply (IHl root_node WFH1 (NatMap.add a s1 k) k' index
-        psi psi' F V C R F' V' C' R' c enc ranV ranV').
+        psi psi' F V C R F' V' C' R' enc ranV ranV').
         exact WFH.
         unfold mlc_deallocation. exact H.
         rewrite <- H0. apply NatMapFacts.add_neq_o.
@@ -909,13 +1289,13 @@ Proof.
       {
         destruct lambda.
         rewrite -> WFH1 in IHTREE. discriminate.
-        specialize (WFH3 c0 a (p :: l) IHTREE).
+        specialize (WFH3 c a (p :: l) IHTREE).
         unfold get_cache_ID_path in IHTREE. discriminate.
         specialize (WFH2 p0 a (p :: l) IHTREE).
         injection WFH2; intros; subst p0.
         apply (WFH4 a p l) in IHTREE.
         apply (IHl (cache_node p) IHTREE (NatMap.add a s1 k) k' index
-        psi psi' F V C R F' V' C' R' c enc ranV ranV').
+        psi psi' F V C R F' V' C' R' enc ranV ranV').
         exact WFH.
         unfold mlc_deallocation. exact H.
         rewrite <- H0. apply NatMapFacts.add_neq_o.
@@ -941,8 +1321,9 @@ Proof.
   intros; destruct (get_cache_ID_path lambda h_tree).
   discriminate.
   destruct state; destruct e; discriminate.
-Admitted.
+Qed.
 
+(* WF3 Preservation *)
 Lemma wf3_preservation : forall sigma obs sigma' obs',
   wf3 sigma -> <<sigma; obs>> ===> <<sigma'; obs'>> -> wf3 sigma'.
 Proof.
@@ -951,61 +1332,95 @@ Proof.
   intros; injection H1; intros.
   inversion H0. inversion H19; subst.
   - case_eq (NatMap.find lambda m); intros; subst.
-
-
-
     destruct s.
-    case_eq (V_range v e); intros.
-    assert (V_range v e = Some l1 -> (In c l1 -> ~ In c c0) /\ (In c c0 -> ~In c l1)).
-    apply (H m mu rho p lambda c0 v w s c e l1). reflexivity. exact H4.
-    apply (wf3_mlc_read lambda0 h_tree m e' mu l0 D delta obs0 k lambda (single_level_cache c0 v w s)
-    (single_level_cache F V C R) c0 v w s F V C R c e l1 ranV).
+    case_eq (NatMap.find e v); intros.
+    apply (wf3_mlc_read lambda0 h_tree m e' mu l0 D delta obs0 k lambda (single_level_cache c v w s)
+    (single_level_cache F V C R) c v w s F V C R e r ranV).
     exact H25. exact H36. exact H4. exact H2. reflexivity.
-    reflexivity. exact H5. exact H3. apply H6 in H5. exact H5.
-    apply (wf2_mlc_read_none lambda0 h_tree m e' mu l0 D delta obs0 k lambda (single_level_cache c0 v w s)
-    (single_level_cache F V C R) c0 v w s F V C R e) in H5.
+    reflexivity. exact H5. exact H3.
+    apply (H m mu rho p lambda c v w s e r).
+    reflexivity. exact H4. exact H5.
+    apply (wf2_mlc_read_none lambda0 h_tree m e' mu l0 D delta obs0 k lambda (single_level_cache c v w s)
+    (single_level_cache F V C R) c v w s F V C R e) in H5.
     rewrite -> H3 in H5. discriminate.
     exact H25. exact H36. exact H4. exact H2. reflexivity.
     reflexivity.
     apply (wf_mlc_read_none lambda0 h_tree m e' mu l0 D delta obs0 k lambda) in H4.
     rewrite -> H2 in H4.
     discriminate. exact H25. exact H36.
-  - give_up.
   - case_eq (NatMap.find lambda m); intros; subst.
     destruct s.
-    case_eq (V_range v0 e); intros.
-    assert (V_range v0 e = Some l1 -> (In c l1 -> ~ In c c0) /\ (In c c0 -> ~In c l1)).
-    apply (H m m0 rho p lambda c0 v0 w s c e l1). reflexivity. exact H4.
-    apply (wf3_mlc_write lambda0 h_tree m e' m0 l0 v D obs1 mu k lambda (single_level_cache c0 v0 w s)
-    (single_level_cache F V C R) c0 v0 w s F V C R c e l1 ranV).
+    case_eq (NatMap.find e v); intros.
+    apply (wf3_mlc_alloc lambda0 h_tree r_bar_val e0 m k lambda (single_level_cache c v w s)
+    (single_level_cache F V C R) c v w s F V C R e r ranV).
+    exact H32. exact H42. exact H4. exact H2. reflexivity.
+    reflexivity. exact H5. exact H3.
+    intros. apply (H m mu rho p lambda c v w s e1 l0).
+    reflexivity. exact H4. exact H6.
+    assert (NatMap.find e V = None).
+    apply (wf2_mlc_alloc_none lambda0 h_tree r_bar_val e0 m k lambda (single_level_cache c v w s)
+    (single_level_cache F V C R) c v w s F V C R e).
+    exact H32. exact H42. exact H4. exact H2. reflexivity.
+    reflexivity. exact H5.
+    rewrite -> H6 in H3. discriminate.
+    apply (wf_mlc_alloc_none lambda0 h_tree r_bar_val e0 m k lambda) in H42.
+    rewrite -> H42 in H2.
+    discriminate. exact H32. exact H4.
+  - case_eq (NatMap.find lambda m); intros; subst.
+    destruct s.
+    case_eq (NatMap.find e v0); intros.
+    apply (wf3_mlc_write lambda0 h_tree m e' m0 l0 v D obs1 mu k lambda (single_level_cache c v0 w s)
+    (single_level_cache F V C R) c v0 w s F V C R e r ranV).
     exact H25. exact H36. exact H4. exact H2. reflexivity.
-    reflexivity. exact H5. exact H3. apply H6 in H5. exact H5.
-    apply (wf2_mlc_write_none lambda0 h_tree m e' m0 l0 v D obs1 mu k lambda (single_level_cache c0 v0 w s)
-    (single_level_cache F V C R) c0 v0 w s F V C R) in H5.
-    rewrite -> H5 in H3. discriminate.
-    exact H25. exact H36. exact H4. exact H2. reflexivity. reflexivity.
+    reflexivity. exact H5. exact H3.
+    apply (H m m0 rho p lambda c v0 w s e r).
+    reflexivity. exact H4. exact H5.
+    apply (wf2_mlc_write_none lambda0 h_tree m e' m0 l0 v D obs1 mu k lambda (single_level_cache c v0 w s)
+    (single_level_cache F V C R) c v0 w s F V C R e) in H5.
+    rewrite -> H3 in H5. discriminate.
+    exact H25. exact H36. exact H4. exact H2. reflexivity.
+    reflexivity.
     apply (wf_mlc_write_none lambda0 h_tree m e' m0 l0 v D obs1 mu k lambda) in H4.
-    rewrite -> H4 in H2.
+    rewrite -> H2 in H4.
     discriminate. exact H25. exact H36.
-  - give_up.
-  - apply (H k mu rho p lambda F V C R c e ranV).
+  - case_eq (NatMap.find lambda m); intros; subst.
+    destruct s.
+    case_eq (NatMap.find e v); intros.
+    apply (wf3_mlc_dealloc lambda0 h_tree (enclave_state_value (enclave_ID_active e_raw) mem) m k lambda (single_level_cache c v w s)
+    (single_level_cache F V C R) c v w s F V C R e r ranV).
+    exact H30. exact H37. exact H4. exact H2. reflexivity.
+    reflexivity. exact H5. exact H3.
+    intros. apply (H m m0 rho p lambda c v w s e0 l0).
+    reflexivity. exact H4. exact H6.
+    assert (NatMap.find e V = None).
+    apply (wf2_mlc_dealloc_none lambda0 h_tree (enclave_state_value (enclave_ID_active e_raw) mem) m k lambda (single_level_cache c v w s)
+    (single_level_cache F V C R) c v w s F V C R e).
+    exact H30. exact H37. exact H4. exact H2.
+    reflexivity. reflexivity. exact H5.
+    rewrite -> H6 in H3. discriminate.
+    apply (wf_mlc_dealloc_none lambda0 h_tree (enclave_state_value (enclave_ID_active e_raw) mem) m k lambda) in H37.
+    rewrite -> H37 in H2.
+    discriminate. exact H30. exact H4.
+  - apply (H k mu rho p lambda F V C R e ranV).
     reflexivity. exact H2. exact H3.
-  - apply (H k mu rho p lambda F V C R c e ranV).
+  - apply (H k mu rho p lambda F V C R e ranV).
     reflexivity. exact H2. exact H3.
-  - apply (H k mu rho p lambda F V C R c e ranV).
+  - apply (H k mu rho p lambda F V C R e ranV).
     reflexivity. exact H2. exact H3.
-  - apply (H k mu rho p lambda F V C R c e ranV).
+  - apply (H k mu rho p lambda F V C R e ranV).
     reflexivity. exact H2. exact H3.
-  - subst. apply (H k mu rho p lambda F V C R c e ranV).
+  - subst; apply (H k mu rho p lambda F V C R e ranV).
     reflexivity. exact H2. exact H3.
-Admitted.
+Qed.
 
+(* Well-Formed 4 *)
 Definition wf4 (sigma: runtime_state): Prop :=
   forall k mu rho pi p l q e E,
   (sigma = runtime_state_value k mu rho pi) ->
   (NatMap.find p pi = Some (process_value (enclave_state_value e E) l q)) ->
   (e = enclave_ID_inactive \/ (exists raw_e, e = enclave_ID_active raw_e /\ NatMap.In raw_e E)).
 
+(* WF4 Active Enclave Update *)
 Lemma wf4_active_enclave_update : forall e E e' E' r,
   active_enclave_update (enclave_state_value e E) r = 
   enclave_state_valid (enclave_state_value e' E') ->
@@ -1032,6 +1447,7 @@ Proof.
   left; reflexivity.
 Qed.
 
+(* WF4 Enclave Creation *)
 Lemma wf4_enclave_creation : forall e E e' E' mu n x y,
   enclave_creation (enclave_state_value e E) mu n x y = enclave_state_valid (enclave_state_value e' E') ->
   (e = enclave_ID_inactive \/ (exists raw_e, e = enclave_ID_active raw_e /\ NatMap.In raw_e E)) ->
@@ -1073,6 +1489,7 @@ Proof.
   discriminate.
 Qed.
 
+(* WF4 Enclave Elimination *)
 Lemma wf4_enclave_elimination : forall e E e' E' r,
   ((enclave_elimination (enclave_state_value e E) r) = enclave_state_valid (enclave_state_value e' E')) ->
   (e = enclave_ID_inactive \/ (exists raw_e, e = enclave_ID_active raw_e /\ NatMap.In raw_e E)) ->
@@ -1127,6 +1544,7 @@ Proof.
   injection H; intros; subst; reflexivity.
 Qed.
 
+(* WF4 Preservation *)
 Lemma wf4_preservation : forall sigma obs sigma' obs',
   wf4 sigma -> <<sigma; obs>> ===> <<sigma'; obs'>> -> wf4 sigma'.
 Proof.
@@ -1304,6 +1722,7 @@ Proof.
     rewrite <- H4. exact H2.
 Qed.
 
+(* Well-Formed 5 *)
 Definition wf5 (sigma: runtime_state): Prop :=
   forall k mu rho pi index F V C R p l q e E,
   (sigma = runtime_state_value k mu rho pi) ->
@@ -1311,6 +1730,260 @@ Definition wf5 (sigma: runtime_state): Prop :=
   (NatMap.find p pi = Some (process_value (enclave_state_value (enclave_ID_active e) E) l q)) ->
   (NatMap.In e V).
 
+(* WF5 MLC Read *)
+Lemma mlc_read_v : forall lambda h_tree k e' m0 l0 D obs1 mu k' index F V C R F' V' C' R',
+  well_defined_cache_tree h_tree ->
+  mlc_read k e' m0 l0 lambda h_tree = mlc_read_valid D obs1 mu k' ->
+  NatMap.find index k = Some (single_level_cache F V C R) ->
+  NatMap.find index k' = Some (single_level_cache F' V' C' R') ->
+  V = V'.
+Proof.
+  unfold mlc_read.
+  intros lambda h_tree.
+  case_eq (get_cache_ID_path lambda h_tree).
+  intros l.
+  generalize dependent lambda.
+  induction l.
+  {
+    intros.
+    unfold recursive_mlc_read in H1.
+    destruct l0. destruct (NatMap.find b m0).
+    injection H1; intros; subst.
+    rewrite -> H2 in H3.
+    injection H3; intros; subst F' V' C' R'.
+    reflexivity.
+    discriminate.
+  }
+  {
+    intros.
+    unfold recursive_mlc_read in H1.
+    fold recursive_mlc_read in H1.
+    case_eq (NatMap.find a k). intros.
+    assert (A0 := H4). destruct (NatMap.find a k) in A0, H1.
+    injection A0; intros; subst s0.
+    case_eq (cc_hit_read s e' l0). intros.
+    assert (A1 := H5). destruct (cc_hit_read s e' l0) in A1, H1.
+    injection A1; injection H1; intros; subst; clear A0 A1.
+    destruct s; destruct s0.
+    apply (cc_hit_read_v (single_level_cache c0 v w s) e' l0 d d0 c
+    (single_level_cache c1 v0 w0 s0) c0 v w s c1 v0 w0 s0) in H5.
+    subst v0.
+    {
+      case_eq (eqb index a); intros.
+      {
+        apply cmp_to_eq in H5; subst a.
+        rewrite -> H2 in H4.
+        injection H4; intros; subst c0 v w s.
+        assert (Some (single_level_cache F' V' C' R') = Some (single_level_cache c1 V w0 s0)).
+        rewrite <- H3. apply NatMapFacts.add_eq_o; reflexivity.
+        injection H5; intros; subst.
+        reflexivity.
+      }
+      {
+        apply cmp_to_uneq in H5.
+        assert (NatMap.find index k = Some (single_level_cache F' V' C' R')).
+        rewrite <- H3. apply eq_sym.
+        apply NatMapFacts.add_neq_o; apply not_eq_sym; exact H5.
+        rewrite -> H2 in H6.
+        injection H6; intros; subst.
+        reflexivity.
+      }
+    }
+    reflexivity.
+    reflexivity.
+    discriminate.
+    intros; destruct (cc_hit_read s e' l0).
+    discriminate.
+    clear A0.
+    case_eq (recursive_mlc_read k e' m0 l0 l); intros.
+    assert (A0 := H6). destruct (recursive_mlc_read k e' m0 l0 l) in A0, H1.
+    case_eq (cc_update s e' d1 l0); intros.
+    assert (A1 := H7). destruct (cc_update s e' d1 l0) in A1, H1.
+    injection A0; injection A1; injection H1; intros; subst; clear A0 A1.
+    {
+      case_eq (eqb index a); intros.
+      {
+        apply cmp_to_eq in H8. subst a.
+        destruct s. rewrite -> H2 in H4; injection H4; intros; subst c0 v w s.
+        destruct s0.
+        apply (cc_update_v (single_level_cache F V C R) e' d l0 c (single_level_cache c0 v w s)
+        F V C R c0 v w s) in H7.
+        subst v.
+        assert (NatMap.find index (NatMap.add index (single_level_cache c0 V w s) m) =
+        Some (single_level_cache c0 V w s)).
+        apply NatMapFacts.add_eq_o. reflexivity.
+        rewrite -> H3 in H7; injection H7; intros; subst c0 V' w s.
+        reflexivity.
+        reflexivity.
+        reflexivity.
+      }
+      {
+        apply cmp_to_uneq in H8.
+        assert (WFH := H0).
+        unfold well_defined_cache_tree in H0.
+        destruct H0 as [ WFH1 ]. destruct H0 as [ WFH2 ]. destruct H0 as [ WFH3 ].
+        destruct l.
+        {
+          apply (IHl root_node WFH1 k e' m0 l0 d d0 o m index F V C R F' V' C' R').
+          exact WFH. exact H6. exact H2.
+          rewrite <- H3. apply eq_sym.
+          apply NatMapFacts.add_neq_o.
+          apply not_eq_sym. exact H8.
+        }
+        {
+          destruct lambda.
+          rewrite -> WFH1 in H. discriminate.
+          specialize (WFH3 c0 a (p :: l) H).
+          unfold get_cache_ID_path in H. discriminate.
+          specialize (WFH2 p0 a (p :: l) H).
+          injection WFH2; intros; subst.
+          apply (H0 p0 p l) in H.
+          apply (IHl (cache_node p) H k e' m0 l0 d d0 o m index F V C R F' V' C' R').
+          exact WFH. exact H6. exact H2.
+          rewrite <- H3. apply eq_sym.
+          apply NatMapFacts.add_neq_o.
+          apply not_eq_sym. exact H8.
+        }
+      }
+    }
+    discriminate.
+    destruct (cc_update s e' d1 l0); discriminate.
+    discriminate.
+    destruct (recursive_mlc_read k e' m0 l0 l); discriminate.
+    discriminate.
+    intros; destruct (NatMap.find a k); discriminate.
+  }
+  intros; destruct (get_cache_ID_path lambda h_tree); discriminate.
+Qed.
+
+(* WF5 MLC Write *)
+Lemma mlc_write_v : forall lambda h_tree k e' m0 l0 v D obs1 mu k' index F V C R F' V' C' R',
+  well_defined_cache_tree h_tree ->
+  mlc_write k e' m0 l0 v lambda h_tree = mlc_write_valid D obs1 mu k' ->
+  NatMap.find index k = Some (single_level_cache F V C R) ->
+  NatMap.find index k' = Some (single_level_cache F' V' C' R') ->
+  V = V'.
+Proof.
+  unfold mlc_write.
+  intros lambda h_tree.
+  case_eq (get_cache_ID_path lambda h_tree).
+  intros l.
+  generalize dependent lambda.
+  induction l.
+  {
+    intros.
+    unfold recursive_mlc_write in H1.
+    destruct l0. destruct (NatMap.find b m0). destruct v.
+    discriminate.
+    injection H1; intros; subst.
+    rewrite -> H2 in H3.
+    injection H3; intros; subst F' V' C' R'.
+    reflexivity.
+    discriminate.
+  }
+  {
+    intros.
+    unfold recursive_mlc_write in H1.
+    fold recursive_mlc_write in H1.
+    case_eq (NatMap.find a k). intros.
+    assert (A0 := H4). destruct (NatMap.find a k) in A0, H1.
+    injection A0; intros; subst s0.
+    case_eq (cc_hit_write s e' l0 v). intros.
+    assert (A1 := H5). destruct (cc_hit_write s e' l0 v) in A1, H1.
+    destruct l0. injection A1; injection H1; intros; subst; clear A0 A1.
+    destruct s; destruct s0.
+    apply (cc_hit_write_v (single_level_cache c0 v0 w s) e' (address b d1) v d c
+    (single_level_cache c1 v1 w0 s0) c0 v0 w s c1 v1 w0 s0) in H5.
+    subst v1.
+    {
+      case_eq (eqb index a); intros.
+      {
+        apply cmp_to_eq in H5; subst a.
+        rewrite -> H2 in H4.
+        injection H4; intros; subst.
+        assert (Some (single_level_cache F' V' C' R') = Some (single_level_cache c1 v0 w0 s0)).
+        rewrite <- H3. apply NatMapFacts.add_eq_o; reflexivity.
+        injection H5; intros; subst.
+        reflexivity.
+      }
+      {
+        apply cmp_to_uneq in H5.
+        assert (NatMap.find index k = Some (single_level_cache F' V' C' R')).
+        rewrite <- H3. apply eq_sym.
+        apply NatMapFacts.add_neq_o; apply not_eq_sym; exact H5.
+        rewrite -> H2 in H6.
+        injection H6; intros; subst.
+        reflexivity.
+      }
+    }
+    reflexivity.
+    reflexivity.
+    discriminate.
+    intros; destruct (cc_hit_write s e' l0 v).
+    discriminate.
+    clear A0.
+    case_eq (recursive_mlc_write k e' m0 l0 v l); intros.
+    assert (A0 := H6). destruct (recursive_mlc_write k e' m0 l0 v l) in A0, H1.
+    case_eq (cc_update s e' d0 l0); intros.
+    assert (A1 := H7). destruct (cc_update s e' d0 l0) in A1, H1.
+    injection A0; injection A1; injection H1; intros; subst; clear A0 A1.
+    {
+      case_eq (eqb index a); intros.
+      {
+        apply cmp_to_eq in H8. subst a.
+        destruct s. rewrite -> H2 in H4; injection H4; intros; subst c0 v0 w s.
+        destruct s0.
+        apply (cc_update_v (single_level_cache F V C R) e' d l0 c (single_level_cache c0 v0 w s)
+        F V C R c0 v0 w s) in H7.
+        subst v0.
+        assert (NatMap.find index (NatMap.add index (single_level_cache c0 V w s) m1) =
+        Some (single_level_cache c0 V w s)).
+        apply NatMapFacts.add_eq_o. reflexivity.
+        rewrite -> H3 in H7; injection H7; intros; subst c0 V' w s.
+        reflexivity.
+        reflexivity.
+        reflexivity.
+      }
+      {
+        apply cmp_to_uneq in H8.
+        assert (WFH := H0).
+        unfold well_defined_cache_tree in H0.
+        destruct H0 as [ WFH1 ]. destruct H0 as [ WFH2 ]. destruct H0 as [ WFH3 ].
+        destruct l.
+        {
+          apply (IHl root_node WFH1 k e' m0 l0 v d o m m1 index F V C R F' V' C' R').
+          exact WFH. exact H6. exact H2.
+          rewrite <- H3. apply eq_sym.
+          apply NatMapFacts.add_neq_o.
+          apply not_eq_sym. exact H8.
+        }
+        {
+          destruct lambda.
+          rewrite -> WFH1 in H. discriminate.
+          specialize (WFH3 c0 a (p :: l) H).
+          unfold get_cache_ID_path in H. discriminate.
+          specialize (WFH2 p0 a (p :: l) H).
+          injection WFH2; intros; subst.
+          apply (H0 p0 p l) in H.
+          apply (IHl (cache_node p) H k e' m0 l0 v d o m m1 index F V C R F' V' C' R').
+          exact WFH. exact H6. exact H2.
+          rewrite <- H3. apply eq_sym.
+          apply NatMapFacts.add_neq_o.
+          apply not_eq_sym. exact H8.
+        }
+      }
+    }
+    discriminate.
+    destruct (cc_update s e' d0 l0); discriminate.
+    discriminate.
+    destruct (recursive_mlc_write k e' m0 l0 v l); discriminate.
+    discriminate.
+    intros; destruct (NatMap.find a k); discriminate.
+  }
+  intros; destruct (get_cache_ID_path lambda h_tree); discriminate.
+Qed.
+
+(* WF5 Preservation *)
 Lemma wf5_preservation : forall sigma obs sigma' obs',
   wf5 sigma -> <<sigma; obs>> ===> <<sigma'; obs'>> -> wf5 sigma'.
 Proof.
@@ -1318,11 +1991,63 @@ Proof.
   unfold wf5 in *.
   intros; injection H1; intros.
   inversion H0. inversion H19.
+  - subst.
+    case_eq (NatMap.find index m); intros. destruct s.
+    apply (mlc_read_v lambda h_tree m e' mu l1 D delta obs0 k index c v w s F V C R) in H36.
+    subst v.
+    case_eq (eqb p1 p2); intros.
+    apply cmp_to_eq in H5; subst p2.
+    assert (Some (process_value (enclave_state_value (enclave_ID_active e) E) l q) =
+    Some (process_value e' l' q0)).
+    rewrite <- H3. apply NatMapFacts.add_eq_o; reflexivity.
+    injection H5; intros; subst.
+    apply (H m mu rho p index c V w s p1 l0 q0 e E).
+    reflexivity. exact H4. exact H20.
+    apply cmp_to_uneq in H5.
+    apply (H m mu rho p index c V w s p1 l q e E).
+    reflexivity. exact H4.
+    rewrite <- H3. apply eq_sym.
+    apply NatMapFacts.add_neq_o; apply not_eq_sym; exact H5.
+    exact H25. exact H4. exact H2.
+    apply (wf_mlc_read_none lambda h_tree m e' mu l1 D delta obs0 k index) in H4.
+    rewrite -> H2 in H4.
+    discriminate. exact H25. exact H36.
   - subst. give_up.
+  - subst.
+    case_eq (NatMap.find index m); intros. destruct s.
+    apply (mlc_write_v lambda h_tree m e' m0 l1 v D obs1 mu k index c v0 w s F V C R) in H36.
+    subst v0.
+    case_eq (eqb p1 p2); intros.
+    apply cmp_to_eq in H5; subst p2.
+    assert (Some (process_value (enclave_state_value (enclave_ID_active e) E) l q) =
+    Some (process_value e' l' q0)).
+    rewrite <- H3. apply NatMapFacts.add_eq_o; reflexivity.
+    injection H5; intros; subst.
+    apply (H m m0 rho p index c V w s p1 l0 q0 e E).
+    reflexivity. exact H4. exact H20.
+    apply cmp_to_uneq in H5.
+    apply (H m m0 rho p index c V w s p1 l q e E).
+    reflexivity. exact H4.
+    rewrite <- H3. apply eq_sym.
+    apply NatMapFacts.add_neq_o; apply not_eq_sym; exact H5.
+    exact H25. exact H4. exact H2.
+    apply (wf_mlc_write_none lambda h_tree m e' m0 l1 v D obs1 mu k index) in H4.
+    rewrite -> H2 in H4.
+    discriminate. exact H25. exact H36.
   - subst. give_up.
-  - subst. give_up.
-  - subst. give_up.
-  - subst. give_up.
+  - subst. case_eq (eqb p1 p2); intros.
+    apply cmp_to_eq in H4; subst p2.
+    assert (Some (process_value (enclave_state_value (enclave_ID_active e) E) l q)
+    = Some (process_value e' l' q0)).
+    rewrite <- H3. apply NatMapFacts.add_eq_o; reflexivity.
+    apply (H k mu rho p index F V C R p1 l q e E).
+    reflexivity. exact H2.
+    give_up.
+    apply cmp_to_uneq in H4.
+    apply (H k mu rho p index F V C R p1 l q e E).
+    reflexivity. exact H2.
+    rewrite <- H3. apply eq_sym.
+    apply NatMapFacts.add_neq_o; apply not_eq_sym; exact H4.
   - subst. give_up.
   - subst. give_up.
   - subst. give_up.
