WellFormed3.v
@@ -1,0 +1,30 @@
+From Coq Require Import Lists.List.
+From Coq Require Import Bool.Bool.
+From Coq Require Import Lia.
+From Coq Require Import FSets.FMapList.
+From Coq Require Import FSets.FMapFacts.
+From Coq Require Import Init.Nat.
+From Coq Require Import Structures.OrderedTypeEx.
+Require Import RuntimeDefinitions.
+Require Import AppendixD.
+Require Import AppendixC.
+Require Import AppendixF.
+Require Import AppendixE.
+Require Import Semantics.
+Require Import MLCOperations.
+Require Import WellFormed.
+
+Module NatMapFacts := NatMapProperties.F.
+Module CacheletMapFacts := CacheletMapProperties.F.
+
+(* Well-Formed 6 *)
+Definition wf6 (sigma: runtime_state): Prop :=
+  forall k mu rho pi lambda F V C R p state E l0 q e l k_num l0 b0 delta0 D0,
+  (sigma = runtime_state_value k mu rho pi) ->
+  NatMap.find p pi = Some (process_value (enclave_state_value state E) l0 q) ->
+  NatMap.find e E = Some (enclave_address_and_data l k_num) ->
+  l0 = memory_address b0 delta0 -> NatMap.find b0 mu = Some D0
+  (exists i, NatMap.find delta0 D0 = Some (memory_value_instruction i)) /\
+  (forall n l' b' delta' D', n < k -> l' = add_to_memory_address mu l n -> l' = memory_address b' delta' ->
+  NatMap.find b' mu = Some D' -> exists n_k, NatMap.find delta' D' = Some (memory_value_data n_k)).
+  
